src/demo/flasher/NotAutomat.thy
@@ -1,19 +1,18 @@
 theory NotAutomat
 
-imports automaton.dAutomaton_causal notAutomat_inc emptychanData
+imports automaton.dAutomaton_causal notAutomat_inc
 
 begin
 (*Not automaton*)
-fun dAnot_transition::"S_not \<Rightarrow> (bool) \<Rightarrow> (S_not \<times> bool)"where
-"dAnot_transition S (bool) = (S,(\<not>bool))"
-
+fun dAnot_transition::"S_not \<Rightarrow> (bool option) \<Rightarrow> (S_not \<times> bool option)"where
+"dAnot_transition S (Some bool) = (S,(Some (\<not>bool)))" |
+"dAnot_transition S (None) = (S,(None))"
 
 interpretation not_smap:smapGen "dAnot_transition" Single "buildNotinSBE" "buildNotoutSBE" Single
   apply(unfold_locales)
-  apply auto[1]
-  done
+  using S_not.exhaust by auto
 
-definition "notStrong  \<equiv>  daw2das not_smap.da (notOutSBE.setter True)"
+definition "notStrong  \<equiv>  daw2das not_smap.da (notOutSBE.setter (Some True))"
 
 abbreviation notStep::"(S_not \<Rightarrow> (inNot\<^sup>\<Omega> \<rightarrow> outNot\<^sup>\<Omega>))"where
 "notStep \<equiv> dawStateSem not_smap.da"
@@ -30,10 +29,13 @@ lemma notoutgetset_eq:"notOutSBE.getterSB\<cdot> (notOutSBE.setterSB\<cdot>s) = 
 lemma notstep2smap:"notOutSBE.getterSB\<cdot>(notStep state\<cdot>(notInSBE.setterSB\<cdot>input)) = (smap not_smap.smapTransition)\<cdot>input"
   by (metis (mono_tags, lifting) S_not.exhaust not_smap.daut2smap somechannotempty)
 
-lemma "notOutSBE.getterSB\<cdot>(notSpf\<cdot>(notInSBE.setterSB\<cdot>input)) = \<up>True \<bullet>(smap not_smap.smapTransition)\<cdot>input"
+lemma "notOutSBE.getterSB\<cdot>(notSpf\<cdot>(notInSBE.setterSB\<cdot>input)) = \<up>(Some True) \<bullet>(smap not_smap.smapTransition)\<cdot>input"
   by(simp add: notSpf_def dasSem_def dasinitout_well das2daw_trunc_well dawSem_def notstep2smap notStrong_def daw2das_def)
 
-lemma not_step:"smap not_smap.smapTransition\<cdot>(\<up>bool \<bullet> s) = \<up>(\<not>bool) \<bullet> smap not_smap.smapTransition\<cdot>s"
+lemma not_step_t1:"smap not_smap.smapTransition\<cdot>(\<up>(Some bool) \<bullet> s) = \<up>(Some (\<not>bool)) \<bullet> smap not_smap.smapTransition\<cdot>s"
+  by simp
+
+lemma not_step_t2:"smap not_smap.smapTransition\<cdot>(\<up>(None) \<bullet> s) = \<up>(None) \<bullet> smap not_smap.smapTransition\<cdot>s"
   by simp
 
 end
